src/program_logic/staged_invariant.v
@@ -1,100 +1,220 @@
-From iris.algebra Require Import gmap auth agree gset coPset excl.
+From iris.algebra Require Import gmap auth agree gset coPset excl csum.
 From iris.base_logic.lib Require Export fancy_updates.
 From stdpp Require Export namespaces.
 From iris.base_logic.lib Require Import wsat invariants saved_prop.
 From iris.algebra Require Import gmap.
 From iris.proofmode Require Import tactics.
+From Perennial.program_logic Require Export step_fupd_extra.
 Set Default Proof Using "Type".
 Import uPred.
 
+Definition crashR := csumR (exclR unitO) (agreeR unitO).
+Definition NC_tok : crashR := Cinl (Excl ()).
+Definition C_tok : crashR := Cinr (to_agree ()).
+
+Class crashG Σ := { crash_inG :> inG Σ crashR; crash_name : gname }.
+
+Definition NC_def `{crashG Σ} := own crash_name NC_tok.
+Definition NC_aux `{crashG Σ} : seal NC_def. by eexists. Qed.
+Definition NC `{crashG Σ} := NC_aux.(unseal).
+Definition C_def `{crashG Σ} := own crash_name C_tok.
+Definition C_aux `{crashG Σ} : seal C_def. by eexists. Qed.
+Definition C `{crashG Σ} := C_aux.(unseal).
+
+
 Class stagedG (Σ : gFunctors) : Set := WsatG {
   staging_saved_inG :> savedPropG Σ;
-  staging_auth_inG :> inG Σ (authR (optionUR (exclR gnameO)));
+  staging_auth_inG :> inG Σ (authR (optionUR (exclR (prodO gnameO gnameO))));
+  staging_shot_inG :> inG Σ (csumR (exclR unitO) (agreeR unitO));
 }.
 
-Definition staged_inv `{!invG Σ, !stagedG Σ} (N: namespace) (γ: gname) (Q: iProp Σ) : iProp Σ :=
-  (inv N (∃ γprop P, own γ (● Excl' γprop) ∗ saved_prop_own γprop P ∗ P ∗ □ (P -∗ Q)))%I.
+Definition staged_pending `{stagedG Σ} (γ: gname) : iProp Σ :=
+  own γ (Cinl (Excl ())).
+Definition staged_done `{stagedG Σ} (γ: gname) : iProp Σ :=
+  own γ (Cinr (to_agree ())).
 
-Definition staged_value `{!stagedG Σ} (N: namespace) (γ: gname) (Q: iProp Σ) : iProp Σ :=
-  (∃ γprop, own γ (◯ Excl' γprop) ∗ saved_prop_own γprop Q)%I.
+Definition staged_inv `{!invG Σ, !crashG Σ, !stagedG Σ} (N: namespace) k E E' (γ γ': gname) (Q: iProp Σ) : iProp Σ :=
+  (inv N (∃ γprop_stored γprop_remainder Ps Pr,
+             own γ (● Excl' (γprop_stored, γprop_remainder)) ∗
+             saved_prop_own γprop_stored Ps ∗
+             saved_prop_own γprop_remainder Pr ∗
+             □ (C -∗ Ps -∗ |={E, E'}_k=> Q ∗ Pr) ∗
+             (Ps ∨ (Pr ∗ C ∗ staged_done γ'))))%I.
+
+Definition staged_value `{!stagedG Σ} (N: namespace) (γ: gname) (Q Q': iProp Σ) : iProp Σ :=
+  (∃ γprop γprop', own γ (◯ Excl' (γprop, γprop')) ∗ saved_prop_own γprop Q ∗ saved_prop_own γprop' Q')%I.
 
 Section inv.
-Context `{!invG Σ, !stagedG Σ}.
+Context `{!invG Σ, !stagedG Σ, !crashG Σ}.
 Implicit Types i : positive.
 Implicit Types N : namespace.
 Implicit Types P Q R : iProp Σ.
 
-Global Instance staged_contractive N γ : Contractive (staged_inv N γ).
-Proof. rewrite /staged_inv. solve_contractive. Qed.
+Global Instance C_timeless : Timeless C.
+Proof. rewrite /C C_aux.(seal_eq). apply _. Qed.
 
-Global Instance staged_ne N γ : NonExpansive (staged_inv N γ).
-Proof. apply contractive_ne, _. Qed.
+Global Instance C_persistent : Persistent C.
+Proof. rewrite /C C_aux.(seal_eq). apply _. Qed.
 
-Global Instance staged_proper N γ : Proper ((⊣⊢) ==> (⊣⊢)) (staged_inv N γ).
+Global Instance NC_timeless : Timeless NC.
+Proof. rewrite /NC NC_aux.(seal_eq). apply _. Qed.
+
+Global Instance staged_contractive N k E E' γ γ' : Contractive (staged_inv N k E E' γ γ').
+Proof.
+  rewrite /staged_inv=> n ?? ?.
+  repeat (apply step_fupdN_ne || f_contractive || f_equiv); eauto.
+Qed.
+
+Global Instance staged_ne N k E E' γ γ': NonExpansive (staged_inv N k E E' γ γ').
+Proof.
+  rewrite /staged_inv=> n ?? ?.
+  repeat (apply step_fupdN_ne || f_contractive || f_equiv); eauto using dist_le.
+Qed.
+
+Global Instance staged_proper N k E E' γ γ' : Proper ((⊣⊢) ==> (⊣⊢)) (staged_inv N k E E' γ γ').
 Proof. apply ne_proper, _. Qed.
 
-Global Instance staged_persistent N γ P : Persistent (staged_inv N γ P).
+Global Instance staged_persistent N k E E' γ γ' P : Persistent (staged_inv N k E E' γ γ' P).
 Proof. rewrite /staged_inv. apply _. Qed.
 
-Lemma staged_inv_iff N γ P Q : ▷ □ (P ↔ Q) -∗ staged_inv N γ P -∗ staged_inv N γ Q.
+Lemma pending_done γ: staged_pending γ -∗ staged_done γ -∗ False.
+Proof.
+  rewrite /staged_pending/staged_done.
+  iIntros "H H'".
+  { by iDestruct (own_valid_2 with "H H'") as %?. }
+Qed.
+
+Lemma pending_upd_done γ: staged_pending γ ==∗ staged_done γ.
+Proof.
+  rewrite /staged_pending/staged_done.
+  iIntros "H". iMod (own_update with "H") as "$".
+  { by apply cmra_update_exclusive. }
+  done.
+Qed.
+
+Lemma staged_inv_iff N k E E' γ γ' P Q :
+  ▷ □ (P ↔ Q) -∗
+  staged_inv N k E E' γ γ' P -∗
+  staged_inv N k E E' γ γ' Q.
 Proof.
   iIntros "#HPQ". iApply inv_iff. iNext. iAlways. iSplit.
-  - iIntros "H". iDestruct "H" as (? P0) "(?&?&?&#HP0)". iExists _, P0. iFrame.
-    iAlways. iIntros. iApply "HPQ". by iApply "HP0".
-  - iIntros "H". iDestruct "H" as (? P0) "(?&?&?&#HP0)". iExists _, P0. iFrame.
-    iAlways. iIntros. iApply "HPQ". by iApply "HP0".
+  - iIntros "H". iDestruct "H" as (?? P0 P0') "(?&?&?&#HP0&Hcase)". iExists _, _, P0, P0'. iFrame.
+    iAlways. iIntros. iSpecialize ("HP0" with "[$] [$]"). 
+    iApply (step_fupdN_inner_wand' with "HP0"); eauto.
+    iIntros "(?&$)". by iApply "HPQ".
+  - iIntros "H". iDestruct "H" as (?? P0 P0') "(?&?&?&#HP0&Hcase)". iExists _, _, P0, P0'. iFrame.
+    iAlways. iIntros. iSpecialize ("HP0" with "[$] [$]").
+    iApply (step_fupdN_inner_wand' with "HP0"); eauto.
+    iIntros "(?&$)". by iApply "HPQ".
 Qed.
 
-Lemma staged_inv_alloc N E P Q: ▷ Q ∗ □ (Q -∗ P) ={E}=∗ ∃ γ, staged_inv N γ P ∗ staged_value N γ Q.
+Lemma staged_inv_alloc N k E E' P Q Qr:
+  ▷ Q ∗ □ (C -∗ Q -∗ P ∗ Qr) ={E}=∗
+  ∃ γ γ', staged_inv N k E' E' γ γ' P ∗ staged_value N γ Q Qr ∗ staged_pending γ'.
 Proof.
   iMod (saved_prop_alloc Q) as (γprop) "#Hsaved".
-  iMod (own_alloc (● (Excl' γprop) ⋅ ◯ (Excl' γprop))) as (γ) "[H1 H2]".
+  iMod (saved_prop_alloc Qr) as (γprop') "#Hsaved'".
+  iMod (own_alloc (● (Excl' (γprop, γprop')) ⋅ ◯ (Excl' (γprop, γprop')))) as (γ) "[H1 H2]".
   { apply auth_both_valid_2; [econstructor | reflexivity]. }
-  iIntros "HP".
-  iMod (inv_alloc N E _ with "[HP H1]") as "HI"; last first.
-  { iModIntro. iExists γ. iSplitL "HI".
+  iMod (own_alloc (Cinl (Excl ()))) as (γ') "H".
+  { econstructor. }
+  iIntros "(HQ&#HQP)".
+  iMod (inv_alloc N E _ with "[HQ H1]") as "HI"; last first.
+  { iModIntro. iExists γ, γ'. iFrame "H". iSplitL "HI".
     - iApply "HI".
-    - iExists γprop. by iFrame.
+    - iExists γprop, γprop'. iFrame. iFrame "#".
   }
-  iNext. iExists γprop, Q. iFrame. auto.
+  iNext. iExists γprop, γprop', Q, Qr. iFrame. iFrame "#".
+  iAlways. iIntros. iApply step_fupdN_inner_later; auto; iNext.
+  iApply "HQP"; by iFrame.
 Qed.
 
-
-Lemma staged_inv_open E N γ P Q:
-  ↑N ⊆ E → staged_inv N γ P ∗ staged_value N γ Q
-           ={E,E∖↑N}=∗ ▷ ▷ Q ∗ (∀ Q', ▷ Q' ∗ □ (Q' -∗ P) ={E∖↑N,E}=∗ staged_value N γ Q').
+Lemma staged_inv_open E N k E1 E2 γ γ' P Q Qr:
+  ↑N ⊆ E →
+  E2 ⊆ E1 →
+  staged_inv N k E1 E2 γ γ' P ∗
+  staged_value N γ Q Qr ={E,E∖↑N}=∗
+  (▷ ▷ Q ∗ (∀ Q' Qr', ▷ Q' ∗ □ (C -∗ Q' -∗ |={E1, E2}_k=> P ∗ Qr') ={E∖↑N,E}=∗ staged_value N γ Q' Qr')) ∨
+  (▷ ▷ Qr ∗ C ∗ |={E∖↑N, E}=> emp).
 Proof.
-  iIntros (?) "(#Hinv&Hval)".
-  iDestruct "Hval" as (γprop) "(Hγ&#Hsaved)".
-  iInv N as (γprop' Qsaved) "H" "HC".
-  iDestruct "H" as "(>Hγ'&#Hsaved'&HQ0&#Himp)".
+  iIntros (??) "(#Hinv&Hval)".
+  iDestruct "Hval" as (γprop γprop') "(Hγ&#Hsaved&#Hsaved')".
+  iInv N as (γprop_alt γprop'_alt Qsaved Qrsaved) "H" "Hclose".
+  iDestruct "H" as "(>Hγ'&#Hsaved_alt&#Hsaved'_alt&HQ0&Hcase)".
   iDestruct (own_valid_2 with "Hγ' Hγ") as "#H".
-  iDestruct "H" as %[<-%Excl_included%leibniz_equiv _]%auth_both_valid.
-  iSplitL "HQ0".
-  - iModIntro. iNext. iDestruct (saved_prop_agree with "Hsaved Hsaved'") as "Hequiv".
-    iNext. by iRewrite "Hequiv".
-  - iModIntro. iIntros (Q'). iIntros "(HQ'&#HQ'impl)".
-    iMod (saved_prop_alloc Q') as (γprop_new) "#Hsaved_new".
-    iMod (own_update_2 _ _ _ (● Excl' γprop_new ⋅ ◯ Excl' γprop_new) with "Hγ' Hγ") as "[Hγ' Hγ]".
-    { by apply auth_update, option_local_update, exclusive_local_update. }
-    iMod ("HC" with "[HQ' Hγ']").
-    * iNext. iExists _, _. iFrame "#". iFrame.
-    * iModIntro. iExists _. by iFrame.
+  iDestruct "H" as %[Heq%Excl_included%leibniz_equiv _]%auth_both_valid.
+  inversion Heq; subst.
+  iDestruct "Hcase" as "[HQ|Hdone]".
+  {
+    iModIntro. iLeft.
+    iSplitL "HQ".
+    - iModIntro.
+      iDestruct (saved_prop_agree with "Hsaved Hsaved_alt") as "Hequiv".
+      iNext. by iRewrite "Hequiv".
+    - iIntros (Q' Qr'). iIntros "(HQ'&#HQ'impl)".
+      iMod (saved_prop_alloc Q') as (γprop_new) "#Hsaved_new".
+      iMod (saved_prop_alloc Qr') as (γprop'_new) "#Hsaved'_new".
+      iMod (own_update_2 _ _ _ (● Excl' (γprop_new, γprop'_new) ⋅
+                                ◯ Excl' (γprop_new, γprop'_new)) with "Hγ' Hγ") as "[Hγ' Hγ]".
+      { by apply auth_update, option_local_update, exclusive_local_update. }
+      iMod ("Hclose" with "[HQ' Hγ']").
+      * iNext. iExists γprop_new, γprop'_new, _, _. iFrame "#". iFrame.
+      * iModIntro. iExists γprop_new, γprop'_new. iFrame "#". iFrame.
+  }
+  {
+    iDestruct "Hdone" as "(HQ&>#HC&>#Hdone)".
+    iModIntro. iRight.
+    iSplitL "HQ".
+    - iModIntro.
+      iDestruct (saved_prop_agree with "Hsaved' Hsaved'_alt") as "Hequiv".
+      iNext. by iRewrite "Hequiv".
+    - iFrame "HC".
+      iMod (saved_prop_alloc P) as (γprop_new) "#Hsaved_new".
+      iMod (saved_prop_alloc True) as (γprop'_new) "#Hsaved'_new".
+      iMod (own_update_2 _ _ _ (● Excl' (γprop_new, γprop'_new) ⋅
+                                ◯ Excl' (γprop_new, γprop'_new)) with "Hγ' Hγ") as "[Hγ' Hγ]".
+      { by apply auth_update, option_local_update, exclusive_local_update. }
+      iMod ("Hclose" with "[Hγ']").
+      * iNext. iExists γprop_new, γprop'_new, _, _. iFrame "#". iFrame.
+        iAlways. iIntros. iApply step_fupdN_inner_later; auto; iNext; by iFrame.
+      * eauto.
+  }
 Qed.
 
-Lemma staged_inv_weak_open E N γ P:
-  ↑N ⊆ E → staged_inv N γ P ={E,E∖↑N}=∗ ▷ P.
+Lemma staged_inv_weak_open E N k E1 γ γ' P:
+  ↑N ⊆ E →
+  E1 ⊆ E ∖ ↑N →
+  staged_inv N k E1 E1 γ γ' P ∗
+  staged_pending γ' ∗
+  C -∗ |={E,E}_(S k)=> P.
 Proof.
-  iIntros (?) "#Hinv".
-  iInv N as (γprop' Qsaved) "H" "HC".
-  iDestruct "H" as "(>Hγ'&#Hsaved'&HQ0&#Himp)".
-  iModIntro. iNext. iApply "Himp". eauto.
+  iIntros (??) "(#Hinv&Hpending&#HC)".
+  iInv N as (γprop_alt γprop'_alt Qsaved Qrsaved) "H" "Hclose".
+  iDestruct "H" as "(>Hγ'&#Hsaved_alt&#Hsaved'_alt&#HQ0&Hcase)".
+  iDestruct "Hcase" as "[HQ|Hfalse]"; last first.
+  { iDestruct "Hfalse" as "(?&?&>H)".
+    iDestruct (pending_done with "[$] [$]") as "[]".
+  }
+  iMod (fupd_intro_mask' _ E1) as "Hclo_E"; first auto.
+  iMod (fupd_intro_mask' _ (∅)) as "Hclo_E1"; first by set_solver.
+  iModIntro. rewrite Nat_iter_S. iModIntro. iNext.
+  iMod "Hclo_E1" as "_".
+  iMod ("HQ0" with "[$] [$]") as "H".
+  iApply (step_fupdN_wand with "H"). iIntros "!> H".
+  iMod "H" as "(HP&HQr)".
+  iMod (pending_upd_done with "[$]") as "#Hdone".
+  iMod "Hclo_E" as "_".
+  iMod ("Hclose" with "[HQr Hγ']").
+  { iNext. iExists _, _, _, _. iFrame "Hγ'". iFrame "#". by iRight. }
+  iModIntro. eauto.
 Qed.
 
+(*
 Global Instance into_inv_staged_inv1 N γ P : IntoInv (staged_inv N γ P) N := {}.
 
 Definition staged_inv_exact N Pweak P :=
   (∃ γ, staged_inv N γ Pweak ∗ staged_value N γ P)%I.
+*)
 
 (*
 Global Instance into_acc_inv E N γ Pweak P :
