src/program_logic/step_fupd_extra.v
@@ -1,0 +1,232 @@
+From iris.proofmode Require Import base tactics classes.
+From iris.base_logic Require Export invariants.
+Set Default Proof Using "Type".
+Import uPred.
+
+Notation "|={ E1 , E2 }_ k => P" :=
+    (|={E1, ∅}=> |={∅, ∅}▷=>^k |={∅, E2}=> P)%I
+      (at level 99, E1, E2 at level 50, k at level 9, P at level 200,
+       format "|={ E1 , E2 }_ k =>  P").
+
+
+Notation "|={ E1 , E2 }_ k =>^ n P" :=
+    (Nat.iter n (λ Q, (|={E1, ∅}=> |={∅, ∅}▷=>^k |={∅, E2}=> Q)) P)%I
+      (at level 99, E1, E2 at level 50, k, n at level 9, P at level 200,
+       format "|={ E1 , E2 }_ k =>^ n  P").
+
+
+Section step_fupdN.
+
+Context {PROP: sbi} {H: BiFUpd PROP} {HAff: BiAffine PROP}.
+
+Lemma step_fupdN_le {E1 E2 : coPset} (n1 n2 : nat) (P: PROP):
+  E2 ⊆ E1 →
+  n1 ≤ n2 → (|={E1,E2}▷=>^n1 P) -∗ |={E1,E2}▷=>^n2 P.
+Proof.
+  intros ?. induction 1 => //=.
+  iIntros. iApply step_fupd_intro; auto. iNext. by iApply IHle.
+Qed.
+
+Lemma step_fupdN_later E1 E2 k (P: PROP):
+  E2 ⊆ E1 →
+  ▷^k P -∗ |={E1,E2}▷=>^k P.
+Proof using HAff.
+  iIntros (Hle).
+  iInduction k as [| k] "IH".
+  - eauto.
+  - iIntros. rewrite Nat_iter_S. iMod (fupd_intro_mask' _ E2) as "Hclo".
+    { set_solver. }
+    iModIntro. iModIntro. iMod "Hclo". iModIntro. by iApply "IH".
+Qed.
+
+Lemma step_fupdN_inner_later E1 E2 k (P: PROP):
+  E2 ⊆ E1 →
+  ▷^k P -∗ |={E1,∅}=> |={∅,∅}▷=>^k |={∅,E2}=> P.
+Proof using HAff.
+  iIntros (Hle).
+  iInduction k as [| k] "IH".
+  - rewrite //=. iIntros "HP".
+    iMod (fupd_intro_mask' _ E2) as "H"; eauto.
+    iApply fupd_intro_mask; eauto; first set_solver.
+  - iIntros. iMod (fupd_intro_mask' _ ∅) as "Hclo".
+    { set_solver. }
+    rewrite Nat_iter_S.
+    iModIntro. iModIntro. iNext. iMod "Hclo". by iApply "IH".
+Qed.
+
+Lemma step_fupdN_inner_fupd E1 E2 k (P: PROP):
+  (|={E1,∅}=> |={∅,∅}▷=>^k |={∅,E2}=> |={E2}=> P) -∗
+  |={E1,∅}=> |={∅,∅}▷=>^k |={∅,E2}=> P.
+Proof.
+  iIntros "H". iMod "H". iApply (step_fupdN_wand with "H").
+  iModIntro. iIntros "H". by iMod "H".
+Qed.
+
+Lemma step_fupdN_inner_plain `{BP: BiPlainly PROP} `{@BiFUpdPlainly PROP H BP}
+      (k: nat) (P: PROP) :
+  Plain P →
+  ((|={⊤, ∅}=> |={∅, ∅}▷=>^k |={∅, ∅}=> P) -∗
+  |={⊤}=> ▷^(S k) P)%I.
+Proof.
+  iIntros (HPlain).
+  iInduction k as [| k] "IH" forall (P HPlain).
+  - rewrite //=. iIntros "H". iApply fupd_plain_mask. do 2 iMod "H".
+    by iModIntro.
+  - iIntros "H".
+    iApply fupd_plain_mask.
+    iMod "H". rewrite -step_fupdN_S_fupd.
+    iMod (step_fupdN_plain with "H") as "H".
+    iModIntro. rewrite -!later_laterN !laterN_later.
+    iNext. iNext. by iMod "H".
+Qed.
+
+Lemma step_fupdN_inner_wand E1 E2 k1 k2 (P Q: PROP):
+  E2 ⊆ E1 →
+  k2 ≤ k1 →
+  (|={E2,∅}=> |={∅,∅}▷=>^k2 |={∅,E2}=> P) -∗
+  (P -∗ Q) -∗
+  |={E1,∅}=> |={∅,∅}▷=>^k1 |={∅,E1}=> Q.
+Proof.
+  iIntros (??) "HP HPQ".
+  iMod (fupd_intro_mask' _ E2) as "Hclo"; auto.
+  iMod "HP". iModIntro.
+  iApply (step_fupdN_le k2 _); auto.
+  iApply (step_fupdN_wand with "HP").
+  iIntros "HP". iMod "HP". iMod "Hclo" as "_".
+  iModIntro. by iApply "HPQ".
+Qed.
+
+Lemma step_fupdN_inner_frame_l E k (P Q: PROP):
+  Q ∗ (|={E,E}_k=> P) -∗ (|={E,E}_k=> Q ∗ P).
+Proof using HAff.
+  iIntros "(HQ&H)". iApply (step_fupdN_inner_wand with "H"); eauto.
+  iIntros; iFrame.
+Qed.
+
+Lemma step_fupdN_inner_frame_r E k (P Q: PROP):
+  (|={E,E}_k=> P) ∗ Q -∗ (|={E,E}_k=> P ∗ Q).
+Proof using HAff.
+  iIntros "(H&HQ)". iApply (step_fupdN_inner_wand with "H"); eauto.
+  iIntros; iFrame.
+Qed.
+
+Lemma step_fupdN_innerN_wand E1 E2 k1 k2 n1 n2 (P Q: PROP):
+  E2 ⊆ E1 →
+  k2 ≤ k1 →
+  n2 ≤ n1 →
+  (|={E2,E2}_k2=>^n2 P) -∗
+  (P -∗ Q) -∗
+  (|={E1,E1}_k1=>^n1 Q).
+Proof using HAff.
+  iIntros (?? Hle) "HP HPQ".
+  iInduction Hle as [] "IH".
+  {
+    iInduction n2 as [|n2] "IH".
+    { iApply "HPQ". eauto. }
+    rewrite !Nat_iter_S.
+    iApply  (step_fupdN_inner_wand with "HP"); auto.
+    iIntros. iApply ("IH" with "[$] [$]").
+  }
+  rewrite Nat_iter_S.
+  iApply (step_fupdN_inner_later); first auto.
+  iNext. by iApply ("IH" with "[$] [$]").
+Qed.
+
+Lemma step_fupdN_inner_wand' E1 E1' E2 E2' k1 k2 (P Q: PROP):
+  E2 ⊆ E1 →
+  E1' ⊆ E2' →
+  k2 ≤ k1 →
+  (|={E2,∅}=> |={∅,∅}▷=>^k2 |={∅,E2'}=> P) -∗
+  (P -∗ Q) -∗
+  |={E1,∅}=> |={∅,∅}▷=>^k1 |={∅,E1'}=> Q.
+Proof using HAff.
+  iIntros (???) "HP HPQ".
+  iMod (fupd_intro_mask' _ E2) as "Hclo"; auto.
+  iMod "HP". iModIntro.
+  iApply (step_fupdN_le k2 _); auto.
+  iApply (step_fupdN_wand with "HP").
+  iIntros "HP". iMod "HP". iApply fupd_mask_weaken; auto.
+  by iApply "HPQ".
+Qed.
+
+Lemma step_fupdN_innerN_wand' E1 E2 k n (P Q: PROP):
+  (|={E1,E2}_k=>^n P) -∗
+  (P -∗ Q) -∗
+  |={E1,E2}_k=>^n Q.
+Proof using HAff.
+  iIntros "HP HPQ". iInduction n as [| n] "IH".
+  - rewrite //=. by iApply "HPQ".
+  - rewrite //=. iApply (step_fupdN_inner_wand' with "HP"); eauto.
+    iIntros; by iApply ("IH" with "[$] [$]").
+Qed.
+
+Lemma step_fupdN_innerN_S_fupd E1 E2 k n (P: PROP):
+  (|={E1,E2}_k=>^(S n) |={E2}=> P) -∗
+  (|={E1,E2}_k=>^(S n) P).
+Proof using HAff.
+  rewrite !Nat_iter_S_r.
+  iIntros "H". iApply (step_fupdN_innerN_wand' with "H").
+  iApply step_fupdN_inner_fupd.
+Qed.
+
+Lemma step_fupdN_inner_plus E1 E2 k1 k2 (P: PROP):
+  (|={E1,∅}=> |={∅,∅}▷=>^k1 |={∅, E1}=> |={E1,∅}=> |={∅,∅}▷=>^k2 |={∅,E2}=> P)
+  ⊢ (|={E1,∅}=> |={∅,∅}▷=>^(k1 + k2) |={∅,E2}=> P)%I.
+Proof using HAff.
+  rewrite Nat_iter_add.
+  iIntros "H". iMod "H". iModIntro.
+  iApply (step_fupdN_mono with "H"). iIntros "H".
+  destruct k2.
+  * simpl. do 3 iMod "H". eauto.
+  * rewrite Nat_iter_S. iMod "H". iMod "H". eauto.
+Qed.
+
+Lemma step_fupdN_ne E1 E2 n:
+  NonExpansive (λ (P: PROP), |={E1, E2}▷=>^n P)%I.
+Proof.
+  induction n => //=.
+  - apply _.
+  - intros ? P Q ->. eauto.
+Qed.
+
+Lemma step_fupdN_inner_plain' `{BP: BiPlainly PROP} `{@BiFUpdPlainly PROP H BP}
+      (k: nat) (P: PROP) :
+  Plain P →
+  ((|={⊤, ⊤}_k=> P) -∗
+  |={⊤}=> ▷^(S k) P)%I.
+Proof using HAff.
+  iIntros (HPlain).
+  iInduction k as [| k] "IH" forall (P HPlain).
+  - rewrite //=. iIntros "H". do 2 iMod "H". eauto.
+  - iIntros "H".
+    iApply (fupd_plain_mask _ ∅).
+    iMod "H".
+    iDestruct (step_fupdN_wand _ _ _ _ (|={∅}=> P)%I with "H []") as "H".
+    { iIntros "H". iMod "H". iApply fupd_mask_weaken; eauto. }
+    rewrite -step_fupdN_S_fupd.
+    iMod (step_fupdN_plain with "H") as "H".
+    iModIntro. rewrite -!later_laterN !laterN_later.
+    iNext. iNext. by iMod "H".
+Qed.
+
+Lemma step_fupdN_innerN_plain `{BP: BiPlainly PROP} `{@BiFUpdPlainly PROP H BP}
+      (k n: nat) (P: PROP) :
+  Plain P →
+  ((|={⊤, ⊤}_k=>^n P) -∗
+  |={⊤}=> ▷^(n * (S k)) P)%I.
+Proof using HAff.
+  iIntros (HPlain).
+  iInduction n as [| n] "IH" forall (P HPlain).
+  - rewrite //=. eauto.
+  - iIntros "H".
+    rewrite Nat_iter_S.
+    iDestruct (step_fupdN_inner_wand with "H []") as "H";
+      [ reflexivity | reflexivity | |].
+    { iApply "IH"; eauto. }
+    rewrite step_fupdN_inner_fupd.
+    iMod (step_fupdN_inner_plain' with "H") as "H".
+    iModIntro. replace (S n * S k) with (S k + (n * S k)) by lia.
+    rewrite laterN_plus; eauto.
+Qed.
+
+End step_fupdN.
